@prefix : <http://www.wordnet.dk/owl/instance/2009/03/concept/> .
@prefix ontolex: <http://www.w3.org/ns/lemon/ontolex#> .
@prefix owl: <http://www.w3.org/2002/07/owl#> .
@prefix rdfs: <http://www.w3.org/2000/01/rdf-schema#> .

:concept a owl:ObjectProperty ;
  rdfs:domain ontolex:LexicalConcept ;
  rdfs:range :Concept ;
  rdfs:comment "The EuroWordNet Concept class of the Synset."@en ;
  rdfs:label "EuroWordNet concept"@en .

:Concept a owl:Class ;
  rdfs:label "EuroWordNet concept"@en ;
  rdfs:comment "A concept based on the 1st, 2nd, and 3rd order entities from EuroWordNet; see: <https://archive.illc.uva.nl/EuroWordNet/corebcs/topont.html>."@en ;
  owl:oneOf (
    :Agentive
    :Animal
    :Artifact
    :Artwork
    :BodyPart
    :BoundedEvent
    :Building
    :Cause
    :Colour
    :Comestible
    :Communication
    :Condition
    :Container
    :Covering
    :Creature
    :Domain
    :Dynamic
    :Existence
    :Experience
    :FirstOrderEntity
    :Form
    :Furniture
    :Garment
    :GeopoliticalPlace
    :Group
    :Human
    :Imagerepresentation
    :Institution
    :Instrument
    :LanguageRepresentation
    :Liquid
    :Living
    :Location
    :Manner
    :Mental
    :MoneyRepresentation
    :Natural
    :Object
    :Occupation
    :Part
    :Phenomenal
    :Physical
    :Place
    :Plant
    :Possession
    :Property
    :Purpose
    :Quantity
    :Relation
    :Representation
    :SecondOrderEntity
    :Social
    :Software
    :Static
    :Stimulating
    :Substance
    :ThirdOrderEntity
    :Time
    :UnboundedEvent
    :Underspecified
    :Vehicle ) .

:Agentive a :Concept ;
  rdfs:label "Agentive"@en ;
  rdfs:comment "The Agentive Concept from EuroWordNet."@en .
:Animal a :Concept ;
  rdfs:label "Animal"@en ;
  rdfs:comment "The Animal Concept from EuroWordNet."@en .
:Artifact a :Concept ;
  rdfs:label "Artifact"@en ;
  rdfs:comment "The Artifact Concept from EuroWordNet."@en .
:Artwork a :Concept ;
  rdfs:label "Artwork"@en ;
  rdfs:comment "The Artwork Concept from EuroWordNet."@en .
:BodyPart a :Concept ;
  rdfs:label "BodyPart"@en ;
  rdfs:comment "The BodyPart Concept from EuroWordNet."@en .
:BoundedEvent a :Concept ;
  rdfs:label "BoundedEvent"@en ;
  rdfs:comment "The BoundedEvent Concept from EuroWordNet."@en .
:Building a :Concept ;
  rdfs:label "Building"@en ;
  rdfs:comment "The Building Concept from EuroWordNet."@en .
:Cause a :Concept ;
  rdfs:label "Cause"@en ;
  rdfs:comment "The Cause Concept from EuroWordNet."@en .
:Colour a :Concept ;
  rdfs:label "Colour"@en ;
  rdfs:comment "The Colour Concept from EuroWordNet."@en .
:Comestible a :Concept ;
  rdfs:label "Comestible"@en ;
  rdfs:comment "The Comestible Concept from EuroWordNet."@en .
:Communication a :Concept ;
  rdfs:label "Communication"@en ;
  rdfs:comment "The Communication Concept from EuroWordNet."@en .
:Condition a :Concept ;
  rdfs:label "Condition"@en ;
  rdfs:comment "The Condition Concept from EuroWordNet."@en .
:Container a :Concept ;
  rdfs:label "Container"@en ;
  rdfs:comment "The Container Concept from EuroWordNet."@en .
:Covering a :Concept ;
  rdfs:label "Covering"@en ;
  rdfs:comment "The Covering Concept from EuroWordNet."@en .
:Creature a :Concept ;
  rdfs:label "Creature"@en ;
  rdfs:comment "The Creature Concept from EuroWordNet."@en .
:Domain a :Concept ;
  rdfs:label "Domain"@en ;
  rdfs:comment "The Domain Concept from EuroWordNet."@en .
:Dynamic a :Concept ;
  rdfs:label "Dynamic"@en ;
  rdfs:comment "The Dynamic Concept from EuroWordNet."@en .
:Existence a :Concept ;
  rdfs:label "Existence"@en ;
  rdfs:comment "The Existence Concept from EuroWordNet."@en .
:Experience a :Concept ;
  rdfs:label "Experience"@en ;
  rdfs:comment "The Experience Concept from EuroWordNet."@en .
:FirstOrderEntity a :Concept ;
  rdfs:label "FirstOrderEntity"@en ;
  rdfs:comment "The FirstOrderEntity Concept from EuroWordNet."@en .
:Form a :Concept ;
  rdfs:label "Form"@en ;
  rdfs:comment "The Form Concept from EuroWordNet."@en .
:Furniture a :Concept ;
  rdfs:label "Furniture"@en ;
  rdfs:comment "The Furniture Concept from EuroWordNet."@en .
:Garment a :Concept ;
  rdfs:label "Garment"@en ;
  rdfs:comment "The Garment Concept from EuroWordNet."@en .
:GeopoliticalPlace a :Concept ;
  rdfs:label "GeopoliticalPlace"@en ;
  rdfs:comment "The GeopoliticalPlace Concept from EuroWordNet."@en .
:Group a :Concept ;
  rdfs:label "Group"@en ;
  rdfs:comment "The Group Concept from EuroWordNet."@en .
:Human a :Concept ;
  rdfs:label "Human"@en ;
  rdfs:comment "The Human Concept from EuroWordNet."@en .
:Imagerepresentation a :Concept ;
  rdfs:label "Imagerepresentation"@en ;
  rdfs:comment "The Imagerepresentation Concept from EuroWordNet."@en .
:Institution a :Concept ;
  rdfs:label "Institution"@en ;
  rdfs:comment "The Institution Concept from EuroWordNet."@en .
:Instrument a :Concept ;
  rdfs:label "Instrument"@en ;
  rdfs:comment "The Instrument Concept from EuroWordNet."@en .
:LanguageRepresentation a :Concept ;
  rdfs:label "LanguageRepresentation"@en ;
  rdfs:comment "The LanguageRepresentation Concept from EuroWordNet."@en .
:Liquid a :Concept ;
  rdfs:label "Liquid"@en ;
  rdfs:comment "The Liquid Concept from EuroWordNet."@en .
:Living a :Concept ;
  rdfs:label "Living"@en ;
  rdfs:comment "The Living Concept from EuroWordNet."@en .
:Location a :Concept ;
  rdfs:label "Location"@en ;
  rdfs:comment "The Location Concept from EuroWordNet."@en .
:Manner a :Concept ;
  rdfs:label "Manner"@en ;
  rdfs:comment "The Manner Concept from EuroWordNet."@en .
:Mental a :Concept ;
  rdfs:label "Mental"@en ;
  rdfs:comment "The Mental Concept from EuroWordNet."@en .
:MoneyRepresentation a :Concept ;
  rdfs:label "MoneyRepresentation"@en ;
  rdfs:comment "The MoneyRepresentation Concept from EuroWordNet."@en .
:Natural a :Concept ;
  rdfs:label "Natural"@en ;
  rdfs:comment "The Natural Concept from EuroWordNet."@en .
:Object a :Concept ;
  rdfs:label "Object"@en ;
  rdfs:comment "The Object Concept from EuroWordNet."@en .
:Occupation a :Concept ;
  rdfs:label "Occupation"@en ;
  rdfs:comment "The Occupation Concept from EuroWordNet."@en .
:Part a :Concept ;
  rdfs:label "Part"@en ;
  rdfs:comment "The Part Concept from EuroWordNet."@en .
:Phenomenal a :Concept ;
  rdfs:label "Phenomenal"@en ;
  rdfs:comment "The Phenomenal Concept from EuroWordNet."@en .
:Physical a :Concept ;
  rdfs:label "Physical"@en ;
  rdfs:comment "The Physical Concept from EuroWordNet."@en .
:Place a :Concept ;
  rdfs:label "Place"@en ;
  rdfs:comment "The Place Concept from EuroWordNet."@en .
:Plant a :Concept ;
  rdfs:label "Plant"@en ;
  rdfs:comment "The Plant Concept from EuroWordNet."@en .
:Possession a :Concept ;
  rdfs:label "Possession"@en ;
  rdfs:comment "The Possession Concept from EuroWordNet."@en .
:Property a :Concept ;
  rdfs:label "Property"@en ;
  rdfs:comment "The Property Concept from EuroWordNet."@en .
:Purpose a :Concept ;
  rdfs:label "Purpose"@en ;
  rdfs:comment "The Purpose Concept from EuroWordNet."@en .
:Quantity a :Concept ;
  rdfs:label "Quantity"@en ;
  rdfs:comment "The Quantity Concept from EuroWordNet."@en .
:Relation a :Concept ;
  rdfs:label "Relation"@en ;
  rdfs:comment "The Relation Concept from EuroWordNet."@en .
:Representation a :Concept ;
  rdfs:label "Representation"@en ;
  rdfs:comment "The Representation Concept from EuroWordNet."@en .
:SecondOrderEntity a :Concept ;
  rdfs:label "SecondOrderEntity"@en ;
  rdfs:comment "The SecondOrderEntity Concept from EuroWordNet."@en .
:Social a :Concept ;
  rdfs:label "Social"@en ;
  rdfs:comment "The Social Concept from EuroWordNet."@en .
:Software a :Concept ;
  rdfs:label "Software"@en ;
  rdfs:comment "The Software Concept from EuroWordNet."@en .
:Static a :Concept ;
  rdfs:label "Static"@en ;
  rdfs:comment "The Static Concept from EuroWordNet."@en .
:Stimulating a :Concept ;
  rdfs:label "Stimulating"@en ;
  rdfs:comment "The Stimulating Concept from EuroWordNet."@en .
:Substance a :Concept ;
  rdfs:label "Substance"@en ;
  rdfs:comment "The Substance Concept from EuroWordNet."@en .
:ThirdOrderEntity a :Concept ;
  rdfs:label "ThirdOrderEntity"@en ;
  rdfs:comment "The ThirdOrderEntity Concept from EuroWordNet."@en .
:Time a :Concept ;
  rdfs:label "Time"@en ;
  rdfs:comment "The Time Concept from EuroWordNet."@en .
:UnboundedEvent a :Concept ;
  rdfs:label "UnboundedEvent"@en ;
  rdfs:comment "The UnboundedEvent Concept from EuroWordNet."@en .
:Underspecified a :Concept ;
  rdfs:label "Underspecified"@en ;
  rdfs:comment "The Underspecified Concept from EuroWordNet."@en .
:Vehicle a :Concept ;
  rdfs:label "Vehicle"@en ;
  rdfs:comment "The Vehicle Concept from EuroWordNet."@en .

:conceptComposite a owl:ObjectProperty ;
  rdfs:domain ontolex:LexicalConcept ;
  rdfs:range :ConceptComposite ;
  rdfs:comment "The EuroWordNet concept composite class of the Synset."@en ;
  rdfs:label "EuroWordNet concept composite"@en .

:ConceptComposite a owl:Class ;
  rdfs:label "EuroWordNet Concept composite"@en ;
  rdfs:comment "A composite of the concepts based on the 1st, 2nd, and 3rd order entities from EuroWordNet; see: <https://archive.illc.uva.nl/EuroWordNet/corebcs/topont.html>."@en ;
  owl:oneOf (
    :Animal-Comestible-Object
    :Animal-Comestible-Part
    :Animal-Comestible-Substance
    :Animal-Object
    :Animal-Object-Group
    :Animal-Object-Part
    :Artifact-Object
    :Artifact-Object-Artwork
    :Artifact-Object-Group
    :Artifact-Object-Part
    :Artifact-Substance
    :Artifact-Substance-Part
    :BoundedEvent
    :BoundedEvent-Agentive
    :BoundedEvent-Agentive-Condition-Physical
    :BoundedEvent-Agentive-Existence
    :BoundedEvent-Agentive-Experience-Condition-Purpose
    :BoundedEvent-Agentive-Mental
    :BoundedEvent-Agentive-Mental-Communication
    :BoundedEvent-Agentive-Mental-Purpose
    :BoundedEvent-Agentive-Physical-Existence
    :BoundedEvent-Agentive-Physical-Existence-Purpose
    :BoundedEvent-Agentive-Physical-Location
    :BoundedEvent-Agentive-Physical-Purpose
    :BoundedEvent-Agentive-Physical-Social
    :BoundedEvent-Agentive-Possession
    :BoundedEvent-Agentive-Purpose
    :BoundedEvent-Agentive-Purpose-Communication
    :BoundedEvent-Agentive-Purpose-Possession
    :BoundedEvent-Agentive-Purpose-Possession-Social
    :BoundedEvent-Agentive-Purpose-Social
    :BoundedEvent-Agentive-Time
    :BoundedEvent-Cause
    :BoundedEvent-Cause-Existence
    :BoundedEvent-Cause-Location-Physical
    :BoundedEvent-Cause-Physical
    :BoundedEvent-Communication
    :BoundedEvent-Experience-Mental
    :BoundedEvent-Experience-Physical
    :BoundedEvent-Location
    :BoundedEvent-Mental
    :BoundedEvent-Phenomenal
    :BoundedEvent-Physical
    :BoundedEvent-Physical-Location
    :BoundedEvent-Possession
    :BoundedEvent-Social
    :Building-Object
    :Building-Object-Group
    :Building-Object-Part
    :Comestible
    :Comestible-Artifact-Liquid
    :Comestible-Artifact-Object
    :Comestible-Artifact-Object-Part
    :Comestible-Artifact-Substance
    :Comestible-Artifact-Substance-Part
    :Comestible-Group
    :Comestible-Natural-Liquid
    :Comestible-Natural-Substance
    :Comestible-Natural-Substance-Part
    :Container-Artifact-Object
    :Container-Artifact-Object-Group
    :Container-Artifact-Object-Part
    :Covering
    :Creature
    :Dynamic
    :Dynamic-Agentive
    :Dynamic-Agentive-Communication
    :Dynamic-Agentive-Mental
    :Dynamic-Agentive-Mental-Purpose
    :Dynamic-Agentive-Physical-Location
    :Dynamic-Agentive-Physical-Purpose
    :Dynamic-Agentive-Physical-Purpose-Social
    :Dynamic-Agentive-Purpose
    :Dynamic-Agentive-Purpose-Social
    :Dynamic-Agentive-Social
    :Dynamic-Cause-Physical
    :Dynamic-Experience
    :Dynamic-Experience-Mental
    :Dynamic-Experience-Physical
    :Dynamic-Phenomenal
    :Dynamic-Phenomenal-Physical
    :Dynamic-Phenomenal-Physical-Condition
    :Dynamic-Possession
    :FirstOrderEntity
    :Form
    :Furniture-Artifact-Object
    :Furniture-Artifact-Object-Group
    :Furniture-Artifact-Object-Part
    :Garment
    :Garment-Artifact-Object
    :Garment-Artifact-Object-Group
    :Garment-Artifact-Object-Part
    :GeopoliticalPlace-Object-Artifact
    :Group
    :Group-Object
    :Group-Object-Living
    :Group-Object-Natural
    :Human-Object
    :Human-Object-Group
    :Human-Object-Occupation
    :Human-Object-Part
    :Imagerepresentation-Artifact-Object
    :Instrument-Artifact-Object
    :Instrument-Artifact-Object-Group
    :Instrument-Artifact-Object-Part
    :LanguageRepresentation-Artifact-Object
    :LanguageRepresentation-Artifact-Object-Group
    :LanguageRepresentation-Artifact-Object-Part
    :Liquid
    :Liquid-Artifact
    :Liquid-Natural
    :Living-Object
    :MoneyRepresentation
    :Natural-Group
    :Natural-Object
    :Natural-Object-BodyPart
    :Natural-Object-Part
    :Natural-Substance
    :Natural-Substance-Part
    :Object
    :Object-Part
    :Part
    :Place
    :Place-Liquid-Natural
    :Place-Object
    :Place-Object-Artifact
    :Place-Object-Artifact-Part
    :Place-Object-Group
    :Place-Object-Natural
    :Place-Object-Natural-Part
    :Place-Object-Part
    :Plant-Group
    :Plant-Object
    :Plant-Object-Comestible
    :Plant-Object-Part
    :Plant-Object-Part-Comestible
    :Property
    :Property-Existence
    :Property-LanguageRepresentation
    :Property-Location
    :Property-Mental
    :Property-Physical
    :Property-Physical-Colour
    :Property-Physical-Condition
    :Property-Physical-Form
    :Property-Social
    :Property-Stimulating-Physical
    :Property-Time
    :Relation
    :Relation-Location
    :Relation-Possession
    :Representation
    :SecondOrderEntity
    :Software
    :Static
    :Static-Existence
    :Static-Location
    :Static-Mental
    :Static-Relation
    :Static-Social
    :Substance
    :ThirdOrderEntity
    :ThirdOrderEntity-Mental
    :ThirdOrderEntity-Mental-Experience
    :ThirdOrderEntity-Mental-Location
    :ThirdOrderEntity-Mental-Purpose
    :ThirdOrderEntity-Mental-Purpose-Domain
    :ThirdOrderEntity-Mental-Purpose-Manner
    :ThirdOrderEntity-Mental-Purpose-Social
    :ThirdOrderEntity-Mental-Purpose-Social-Institution
    :ThirdOrderEntity-Mental-Social
    :ThirdOrderEntity-Part
    :ThirdOrderEntity-Quantity
    :ThirdOrderEntity-Quantity-MoneyRepresentation
    :ThirdOrderEntity-Quantity-Part
    :ThirdOrderEntity-Relation
    :ThirdOrderEntity-Time
    :ThirdOrderEntity-Time-Part
    :UnboundedEvent
    :UnboundedEvent-Agentive
    :UnboundedEvent-Agentive-Communication-Social
    :UnboundedEvent-Agentive-Existence
    :UnboundedEvent-Agentive-Mental
    :UnboundedEvent-Agentive-Physical
    :UnboundedEvent-Agentive-Physical-Location
    :UnboundedEvent-Agentive-Physical-Purpose
    :UnboundedEvent-Agentive-Physical-Social
    :UnboundedEvent-Agentive-Purpose
    :UnboundedEvent-Cause
    :UnboundedEvent-Cause-Physical
    :UnboundedEvent-Cause-Physical-Location
    :UnboundedEvent-Communication-Purpose-Social
    :UnboundedEvent-Experience-Physical
    :UnboundedEvent-Mental
    :UnboundedEvent-Phenomenal
    :UnboundedEvent-Phenomenal-Physical
    :UnboundedEvent-Physical-Location
    :UnboundedEvent-Social
    :UnboundedEvent-Time
    :Underspecified
    :Vehicle-Object-Artifact
    :Vehicle-Object-Artifact-Group
    :Vehicle-Object-Artifact-Part ) .

:Animal-Comestible-Object a :ConceptComposite ;
  rdfs:label "Animal-Comestible-Object"@en ;
  rdfs:comment "The composite of the EuroWordNet Concepts Animal-Comestible-Object."@en .
:Animal-Comestible-Part a :ConceptComposite ;
  rdfs:label "Animal-Comestible-Part"@en ;
  rdfs:comment "The composite of the EuroWordNet Concepts Animal-Comestible-Part."@en .
:Animal-Comestible-Substance a :ConceptComposite ;
  rdfs:label "Animal-Comestible-Substance"@en ;
  rdfs:comment "The composite of the EuroWordNet Concepts Animal-Comestible-Substance."@en .
:Animal-Object a :ConceptComposite ;
  rdfs:label "Animal-Object"@en ;
  rdfs:comment "The composite of the EuroWordNet Concepts Animal-Object."@en .
:Animal-Object-Group a :ConceptComposite ;
  rdfs:label "Animal-Object-Group"@en ;
  rdfs:comment "The composite of the EuroWordNet Concepts Animal-Object-Group."@en .
:Animal-Object-Part a :ConceptComposite ;
  rdfs:label "Animal-Object-Part"@en ;
  rdfs:comment "The composite of the EuroWordNet Concepts Animal-Object-Part."@en .
:Artifact-Object a :ConceptComposite ;
  rdfs:label "Artifact-Object"@en ;
  rdfs:comment "The composite of the EuroWordNet Concepts Artifact-Object."@en .
:Artifact-Object-Artwork a :ConceptComposite ;
  rdfs:label "Artifact-Object-Artwork"@en ;
  rdfs:comment "The composite of the EuroWordNet Concepts Artifact-Object-Artwork."@en .
:Artifact-Object-Group a :ConceptComposite ;
  rdfs:label "Artifact-Object-Group"@en ;
  rdfs:comment "The composite of the EuroWordNet Concepts Artifact-Object-Group."@en .
:Artifact-Object-Part a :ConceptComposite ;
  rdfs:label "Artifact-Object-Part"@en ;
  rdfs:comment "The composite of the EuroWordNet Concepts Artifact-Object-Part."@en .
:Artifact-Substance a :ConceptComposite ;
  rdfs:label "Artifact-Substance"@en ;
  rdfs:comment "The composite of the EuroWordNet Concepts Artifact-Substance."@en .
:Artifact-Substance-Part a :ConceptComposite ;
  rdfs:label "Artifact-Substance-Part"@en ;
  rdfs:comment "The composite of the EuroWordNet Concepts Artifact-Substance-Part."@en .
:BoundedEvent a :ConceptComposite ;
  rdfs:label "BoundedEvent"@en ;
  rdfs:comment "The composite of the EuroWordNet Concepts BoundedEvent."@en .
:BoundedEvent-Agentive a :ConceptComposite ;
  rdfs:label "BoundedEvent-Agentive"@en ;
  rdfs:comment "The composite of the EuroWordNet Concepts BoundedEvent-Agentive."@en .
:BoundedEvent-Agentive-Condition-Physical a :ConceptComposite ;
  rdfs:label "BoundedEvent-Agentive-Condition-Physical"@en ;
  rdfs:comment "The composite of the EuroWordNet Concepts BoundedEvent-Agentive-Condition-Physical."@en .
:BoundedEvent-Agentive-Existence a :ConceptComposite ;
  rdfs:label "BoundedEvent-Agentive-Existence"@en ;
  rdfs:comment "The composite of the EuroWordNet Concepts BoundedEvent-Agentive-Existence."@en .
:BoundedEvent-Agentive-Experience-Condition-Purpose a :ConceptComposite ;
  rdfs:label "BoundedEvent-Agentive-Experience-Condition-Purpose"@en ;
  rdfs:comment "The composite of the EuroWordNet Concepts BoundedEvent-Agentive-Experience-Condition-Purpose."@en .
:BoundedEvent-Agentive-Mental a :ConceptComposite ;
  rdfs:label "BoundedEvent-Agentive-Mental"@en ;
  rdfs:comment "The composite of the EuroWordNet Concepts BoundedEvent-Agentive-Mental."@en .
:BoundedEvent-Agentive-Mental-Communication a :ConceptComposite ;
  rdfs:label "BoundedEvent-Agentive-Mental-Communication"@en ;
  rdfs:comment "The composite of the EuroWordNet Concepts BoundedEvent-Agentive-Mental-Communication."@en .
:BoundedEvent-Agentive-Mental-Purpose a :ConceptComposite ;
  rdfs:label "BoundedEvent-Agentive-Mental-Purpose"@en ;
  rdfs:comment "The composite of the EuroWordNet Concepts BoundedEvent-Agentive-Mental-Purpose."@en .
:BoundedEvent-Agentive-Physical-Existence a :ConceptComposite ;
  rdfs:label "BoundedEvent-Agentive-Physical-Existence"@en ;
  rdfs:comment "The composite of the EuroWordNet Concepts BoundedEvent-Agentive-Physical-Existence."@en .
:BoundedEvent-Agentive-Physical-Existence-Purpose a :ConceptComposite ;
  rdfs:label "BoundedEvent-Agentive-Physical-Existence-Purpose"@en ;
  rdfs:comment "The composite of the EuroWordNet Concepts BoundedEvent-Agentive-Physical-Existence-Purpose."@en .
:BoundedEvent-Agentive-Physical-Location a :ConceptComposite ;
  rdfs:label "BoundedEvent-Agentive-Physical-Location"@en ;
  rdfs:comment "The composite of the EuroWordNet Concepts BoundedEvent-Agentive-Physical-Location."@en .
:BoundedEvent-Agentive-Physical-Purpose a :ConceptComposite ;
  rdfs:label "BoundedEvent-Agentive-Physical-Purpose"@en ;
  rdfs:comment "The composite of the EuroWordNet Concepts BoundedEvent-Agentive-Physical-Purpose."@en .
:BoundedEvent-Agentive-Physical-Social a :ConceptComposite ;
  rdfs:label "BoundedEvent-Agentive-Physical-Social"@en ;
  rdfs:comment "The composite of the EuroWordNet Concepts BoundedEvent-Agentive-Physical-Social."@en .
:BoundedEvent-Agentive-Possession a :ConceptComposite ;
  rdfs:label "BoundedEvent-Agentive-Possession"@en ;
  rdfs:comment "The composite of the EuroWordNet Concepts BoundedEvent-Agentive-Possession."@en .
:BoundedEvent-Agentive-Purpose a :ConceptComposite ;
  rdfs:label "BoundedEvent-Agentive-Purpose"@en ;
  rdfs:comment "The composite of the EuroWordNet Concepts BoundedEvent-Agentive-Purpose."@en .
:BoundedEvent-Agentive-Purpose-Communication a :ConceptComposite ;
  rdfs:label "BoundedEvent-Agentive-Purpose-Communication"@en ;
  rdfs:comment "The composite of the EuroWordNet Concepts BoundedEvent-Agentive-Purpose-Communication."@en .
:BoundedEvent-Agentive-Purpose-Possession a :ConceptComposite ;
  rdfs:label "BoundedEvent-Agentive-Purpose-Possession"@en ;
  rdfs:comment "The composite of the EuroWordNet Concepts BoundedEvent-Agentive-Purpose-Possession."@en .
:BoundedEvent-Agentive-Purpose-Possession-Social a :ConceptComposite ;
  rdfs:label "BoundedEvent-Agentive-Purpose-Possession-Social"@en ;
  rdfs:comment "The composite of the EuroWordNet Concepts BoundedEvent-Agentive-Purpose-Possession-Social."@en .
:BoundedEvent-Agentive-Purpose-Social a :ConceptComposite ;
  rdfs:label "BoundedEvent-Agentive-Purpose-Social"@en ;
  rdfs:comment "The composite of the EuroWordNet Concepts BoundedEvent-Agentive-Purpose-Social."@en .
:BoundedEvent-Agentive-Time a :ConceptComposite ;
  rdfs:label "BoundedEvent-Agentive-Time"@en ;
  rdfs:comment "The composite of the EuroWordNet Concepts BoundedEvent-Agentive-Time."@en .
:BoundedEvent-Cause a :ConceptComposite ;
  rdfs:label "BoundedEvent-Cause"@en ;
  rdfs:comment "The composite of the EuroWordNet Concepts BoundedEvent-Cause."@en .
:BoundedEvent-Cause-Existence a :ConceptComposite ;
  rdfs:label "BoundedEvent-Cause-Existence"@en ;
  rdfs:comment "The composite of the EuroWordNet Concepts BoundedEvent-Cause-Existence."@en .
:BoundedEvent-Cause-Location-Physical a :ConceptComposite ;
  rdfs:label "BoundedEvent-Cause-Location-Physical"@en ;
  rdfs:comment "The composite of the EuroWordNet Concepts BoundedEvent-Cause-Location-Physical."@en .
:BoundedEvent-Cause-Physical a :ConceptComposite ;
  rdfs:label "BoundedEvent-Cause-Physical"@en ;
  rdfs:comment "The composite of the EuroWordNet Concepts BoundedEvent-Cause-Physical."@en .
:BoundedEvent-Communication a :ConceptComposite ;
  rdfs:label "BoundedEvent-Communication"@en ;
  rdfs:comment "The composite of the EuroWordNet Concepts BoundedEvent-Communication."@en .
:BoundedEvent-Experience-Mental a :ConceptComposite ;
  rdfs:label "BoundedEvent-Experience-Mental"@en ;
  rdfs:comment "The composite of the EuroWordNet Concepts BoundedEvent-Experience-Mental."@en .
:BoundedEvent-Experience-Physical a :ConceptComposite ;
  rdfs:label "BoundedEvent-Experience-Physical"@en ;
  rdfs:comment "The composite of the EuroWordNet Concepts BoundedEvent-Experience-Physical."@en .
:BoundedEvent-Location a :ConceptComposite ;
  rdfs:label "BoundedEvent-Location"@en ;
  rdfs:comment "The composite of the EuroWordNet Concepts BoundedEvent-Location."@en .
:BoundedEvent-Mental a :ConceptComposite ;
  rdfs:label "BoundedEvent-Mental"@en ;
  rdfs:comment "The composite of the EuroWordNet Concepts BoundedEvent-Mental."@en .
:BoundedEvent-Phenomenal a :ConceptComposite ;
  rdfs:label "BoundedEvent-Phenomenal"@en ;
  rdfs:comment "The composite of the EuroWordNet Concepts BoundedEvent-Phenomenal."@en .
:BoundedEvent-Physical a :ConceptComposite ;
  rdfs:label "BoundedEvent-Physical"@en ;
  rdfs:comment "The composite of the EuroWordNet Concepts BoundedEvent-Physical."@en .
:BoundedEvent-Physical-Location a :ConceptComposite ;
  rdfs:label "BoundedEvent-Physical-Location"@en ;
  rdfs:comment "The composite of the EuroWordNet Concepts BoundedEvent-Physical-Location."@en .
:BoundedEvent-Possession a :ConceptComposite ;
  rdfs:label "BoundedEvent-Possession"@en ;
  rdfs:comment "The composite of the EuroWordNet Concepts BoundedEvent-Possession."@en .
:BoundedEvent-Social a :ConceptComposite ;
  rdfs:label "BoundedEvent-Social"@en ;
  rdfs:comment "The composite of the EuroWordNet Concepts BoundedEvent-Social."@en .
:Building-Object a :ConceptComposite ;
  rdfs:label "Building-Object"@en ;
  rdfs:comment "The composite of the EuroWordNet Concepts Building-Object."@en .
:Building-Object-Group a :ConceptComposite ;
  rdfs:label "Building-Object-Group"@en ;
  rdfs:comment "The composite of the EuroWordNet Concepts Building-Object-Group."@en .
:Building-Object-Part a :ConceptComposite ;
  rdfs:label "Building-Object-Part"@en ;
  rdfs:comment "The composite of the EuroWordNet Concepts Building-Object-Part."@en .
:Comestible a :ConceptComposite ;
  rdfs:label "Comestible"@en ;
  rdfs:comment "The composite of the EuroWordNet Concepts Comestible."@en .
:Comestible-Artifact-Liquid a :ConceptComposite ;
  rdfs:label "Comestible-Artifact-Liquid"@en ;
  rdfs:comment "The composite of the EuroWordNet Concepts Comestible-Artifact-Liquid."@en .
:Comestible-Artifact-Object a :ConceptComposite ;
  rdfs:label "Comestible-Artifact-Object"@en ;
  rdfs:comment "The composite of the EuroWordNet Concepts Comestible-Artifact-Object."@en .
:Comestible-Artifact-Object-Part a :ConceptComposite ;
  rdfs:label "Comestible-Artifact-Object-Part"@en ;
  rdfs:comment "The composite of the EuroWordNet Concepts Comestible-Artifact-Object-Part."@en .
:Comestible-Artifact-Substance a :ConceptComposite ;
  rdfs:label "Comestible-Artifact-Substance"@en ;
  rdfs:comment "The composite of the EuroWordNet Concepts Comestible-Artifact-Substance."@en .
:Comestible-Artifact-Substance-Part a :ConceptComposite ;
  rdfs:label "Comestible-Artifact-Substance-Part"@en ;
  rdfs:comment "The composite of the EuroWordNet Concepts Comestible-Artifact-Substance-Part."@en .
:Comestible-Group a :ConceptComposite ;
  rdfs:label "Comestible-Group"@en ;
  rdfs:comment "The composite of the EuroWordNet Concepts Comestible-Group."@en .
:Comestible-Natural-Liquid a :ConceptComposite ;
  rdfs:label "Comestible-Natural-Liquid"@en ;
  rdfs:comment "The composite of the EuroWordNet Concepts Comestible-Natural-Liquid."@en .
:Comestible-Natural-Substance a :ConceptComposite ;
  rdfs:label "Comestible-Natural-Substance"@en ;
  rdfs:comment "The composite of the EuroWordNet Concepts Comestible-Natural-Substance."@en .
:Comestible-Natural-Substance-Part a :ConceptComposite ;
  rdfs:label "Comestible-Natural-Substance-Part"@en ;
  rdfs:comment "The composite of the EuroWordNet Concepts Comestible-Natural-Substance-Part."@en .
:Container-Artifact-Object a :ConceptComposite ;
  rdfs:label "Container-Artifact-Object"@en ;
  rdfs:comment "The composite of the EuroWordNet Concepts Container-Artifact-Object."@en .
:Container-Artifact-Object-Group a :ConceptComposite ;
  rdfs:label "Container-Artifact-Object-Group"@en ;
  rdfs:comment "The composite of the EuroWordNet Concepts Container-Artifact-Object-Group."@en .
:Container-Artifact-Object-Part a :ConceptComposite ;
  rdfs:label "Container-Artifact-Object-Part"@en ;
  rdfs:comment "The composite of the EuroWordNet Concepts Container-Artifact-Object-Part."@en .
:Covering a :ConceptComposite ;
  rdfs:label "Covering"@en ;
  rdfs:comment "The composite of the EuroWordNet Concepts Covering."@en .
:Creature a :ConceptComposite ;
  rdfs:label "Creature"@en ;
  rdfs:comment "The composite of the EuroWordNet Concepts Creature."@en .
:Dynamic a :ConceptComposite ;
  rdfs:label "Dynamic"@en ;
  rdfs:comment "The composite of the EuroWordNet Concepts Dynamic."@en .
:Dynamic-Agentive a :ConceptComposite ;
  rdfs:label "Dynamic-Agentive"@en ;
  rdfs:comment "The composite of the EuroWordNet Concepts Dynamic-Agentive."@en .
:Dynamic-Agentive-Communication a :ConceptComposite ;
  rdfs:label "Dynamic-Agentive-Communication"@en ;
  rdfs:comment "The composite of the EuroWordNet Concepts Dynamic-Agentive-Communication."@en .
:Dynamic-Agentive-Mental a :ConceptComposite ;
  rdfs:label "Dynamic-Agentive-Mental"@en ;
  rdfs:comment "The composite of the EuroWordNet Concepts Dynamic-Agentive-Mental."@en .
:Dynamic-Agentive-Mental-Purpose a :ConceptComposite ;
  rdfs:label "Dynamic-Agentive-Mental-Purpose"@en ;
  rdfs:comment "The composite of the EuroWordNet Concepts Dynamic-Agentive-Mental-Purpose."@en .
:Dynamic-Agentive-Physical-Location a :ConceptComposite ;
  rdfs:label "Dynamic-Agentive-Physical-Location"@en ;
  rdfs:comment "The composite of the EuroWordNet Concepts Dynamic-Agentive-Physical-Location."@en .
:Dynamic-Agentive-Physical-Purpose a :ConceptComposite ;
  rdfs:label "Dynamic-Agentive-Physical-Purpose"@en ;
  rdfs:comment "The composite of the EuroWordNet Concepts Dynamic-Agentive-Physical-Purpose."@en .
:Dynamic-Agentive-Physical-Purpose-Social a :ConceptComposite ;
  rdfs:label "Dynamic-Agentive-Physical-Purpose-Social"@en ;
  rdfs:comment "The composite of the EuroWordNet Concepts Dynamic-Agentive-Physical-Purpose-Social."@en .
:Dynamic-Agentive-Purpose a :ConceptComposite ;
  rdfs:label "Dynamic-Agentive-Purpose"@en ;
  rdfs:comment "The composite of the EuroWordNet Concepts Dynamic-Agentive-Purpose."@en .
:Dynamic-Agentive-Purpose-Social a :ConceptComposite ;
  rdfs:label "Dynamic-Agentive-Purpose-Social"@en ;
  rdfs:comment "The composite of the EuroWordNet Concepts Dynamic-Agentive-Purpose-Social."@en .
:Dynamic-Agentive-Social a :ConceptComposite ;
  rdfs:label "Dynamic-Agentive-Social"@en ;
  rdfs:comment "The composite of the EuroWordNet Concepts Dynamic-Agentive-Social."@en .
:Dynamic-Cause-Physical a :ConceptComposite ;
  rdfs:label "Dynamic-Cause-Physical"@en ;
  rdfs:comment "The composite of the EuroWordNet Concepts Dynamic-Cause-Physical."@en .
:Dynamic-Experience a :ConceptComposite ;
  rdfs:label "Dynamic-Experience"@en ;
  rdfs:comment "The composite of the EuroWordNet Concepts Dynamic-Experience."@en .
:Dynamic-Experience-Mental a :ConceptComposite ;
  rdfs:label "Dynamic-Experience-Mental"@en ;
  rdfs:comment "The composite of the EuroWordNet Concepts Dynamic-Experience-Mental."@en .
:Dynamic-Experience-Physical a :ConceptComposite ;
  rdfs:label "Dynamic-Experience-Physical"@en ;
  rdfs:comment "The composite of the EuroWordNet Concepts Dynamic-Experience-Physical."@en .
:Dynamic-Phenomenal a :ConceptComposite ;
  rdfs:label "Dynamic-Phenomenal"@en ;
  rdfs:comment "The composite of the EuroWordNet Concepts Dynamic-Phenomenal."@en .
:Dynamic-Phenomenal-Physical a :ConceptComposite ;
  rdfs:label "Dynamic-Phenomenal-Physical"@en ;
  rdfs:comment "The composite of the EuroWordNet Concepts Dynamic-Phenomenal-Physical."@en .
:Dynamic-Phenomenal-Physical-Condition a :ConceptComposite ;
  rdfs:label "Dynamic-Phenomenal-Physical-Condition"@en ;
  rdfs:comment "The composite of the EuroWordNet Concepts Dynamic-Phenomenal-Physical-Condition."@en .
:Dynamic-Possession a :ConceptComposite ;
  rdfs:label "Dynamic-Possession"@en ;
  rdfs:comment "The composite of the EuroWordNet Concepts Dynamic-Possession."@en .
:FirstOrderEntity a :ConceptComposite ;
  rdfs:label "FirstOrderEntity"@en ;
  rdfs:comment "The composite of the EuroWordNet Concepts FirstOrderEntity."@en .
:Form a :ConceptComposite ;
  rdfs:label "Form"@en ;
  rdfs:comment "The composite of the EuroWordNet Concepts Form."@en .
:Furniture-Artifact-Object a :ConceptComposite ;
  rdfs:label "Furniture-Artifact-Object"@en ;
  rdfs:comment "The composite of the EuroWordNet Concepts Furniture-Artifact-Object."@en .
:Furniture-Artifact-Object-Group a :ConceptComposite ;
  rdfs:label "Furniture-Artifact-Object-Group"@en ;
  rdfs:comment "The composite of the EuroWordNet Concepts Furniture-Artifact-Object-Group."@en .
:Furniture-Artifact-Object-Part a :ConceptComposite ;
  rdfs:label "Furniture-Artifact-Object-Part"@en ;
  rdfs:comment "The composite of the EuroWordNet Concepts Furniture-Artifact-Object-Part."@en .
:Garment a :ConceptComposite ;
  rdfs:label "Garment"@en ;
  rdfs:comment "The composite of the EuroWordNet Concepts Garment."@en .
:Garment-Artifact-Object a :ConceptComposite ;
  rdfs:label "Garment-Artifact-Object"@en ;
  rdfs:comment "The composite of the EuroWordNet Concepts Garment-Artifact-Object."@en .
:Garment-Artifact-Object-Group a :ConceptComposite ;
  rdfs:label "Garment-Artifact-Object-Group"@en ;
  rdfs:comment "The composite of the EuroWordNet Concepts Garment-Artifact-Object-Group."@en .
:Garment-Artifact-Object-Part a :ConceptComposite ;
  rdfs:label "Garment-Artifact-Object-Part"@en ;
  rdfs:comment "The composite of the EuroWordNet Concepts Garment-Artifact-Object-Part."@en .
:GeopoliticalPlace-Object-Artifact a :ConceptComposite ;
  rdfs:label "GeopoliticalPlace-Object-Artifact"@en ;
  rdfs:comment "The composite of the EuroWordNet Concepts GeopoliticalPlace-Object-Artifact."@en .
:Group a :ConceptComposite ;
  rdfs:label "Group"@en ;
  rdfs:comment "The composite of the EuroWordNet Concepts Group."@en .
:Group-Object a :ConceptComposite ;
  rdfs:label "Group-Object"@en ;
  rdfs:comment "The composite of the EuroWordNet Concepts Group-Object."@en .
:Group-Object-Living a :ConceptComposite ;
  rdfs:label "Group-Object-Living"@en ;
  rdfs:comment "The composite of the EuroWordNet Concepts Group-Object-Living."@en .
:Group-Object-Natural a :ConceptComposite ;
  rdfs:label "Group-Object-Natural"@en ;
  rdfs:comment "The composite of the EuroWordNet Concepts Group-Object-Natural."@en .
:Human-Object a :ConceptComposite ;
  rdfs:label "Human-Object"@en ;
  rdfs:comment "The composite of the EuroWordNet Concepts Human-Object."@en .
:Human-Object-Group a :ConceptComposite ;
  rdfs:label "Human-Object-Group"@en ;
  rdfs:comment "The composite of the EuroWordNet Concepts Human-Object-Group."@en .
:Human-Object-Occupation a :ConceptComposite ;
  rdfs:label "Human-Object-Occupation"@en ;
  rdfs:comment "The composite of the EuroWordNet Concepts Human-Object-Occupation."@en .
:Human-Object-Part a :ConceptComposite ;
  rdfs:label "Human-Object-Part"@en ;
  rdfs:comment "The composite of the EuroWordNet Concepts Human-Object-Part."@en .
:Imagerepresentation-Artifact-Object a :ConceptComposite ;
  rdfs:label "Imagerepresentation-Artifact-Object"@en ;
  rdfs:comment "The composite of the EuroWordNet Concepts Imagerepresentation-Artifact-Object."@en .
:Instrument-Artifact-Object a :ConceptComposite ;
  rdfs:label "Instrument-Artifact-Object"@en ;
  rdfs:comment "The composite of the EuroWordNet Concepts Instrument-Artifact-Object."@en .
:Instrument-Artifact-Object-Group a :ConceptComposite ;
  rdfs:label "Instrument-Artifact-Object-Group"@en ;
  rdfs:comment "The composite of the EuroWordNet Concepts Instrument-Artifact-Object-Group."@en .
:Instrument-Artifact-Object-Part a :ConceptComposite ;
  rdfs:label "Instrument-Artifact-Object-Part"@en ;
  rdfs:comment "The composite of the EuroWordNet Concepts Instrument-Artifact-Object-Part."@en .
:LanguageRepresentation-Artifact-Object a :ConceptComposite ;
  rdfs:label "LanguageRepresentation-Artifact-Object"@en ;
  rdfs:comment "The composite of the EuroWordNet Concepts LanguageRepresentation-Artifact-Object."@en .
:LanguageRepresentation-Artifact-Object-Group a :ConceptComposite ;
  rdfs:label "LanguageRepresentation-Artifact-Object-Group"@en ;
  rdfs:comment "The composite of the EuroWordNet Concepts LanguageRepresentation-Artifact-Object-Group."@en .
:LanguageRepresentation-Artifact-Object-Part a :ConceptComposite ;
  rdfs:label "LanguageRepresentation-Artifact-Object-Part"@en ;
  rdfs:comment "The composite of the EuroWordNet Concepts LanguageRepresentation-Artifact-Object-Part."@en .
:Liquid a :ConceptComposite ;
  rdfs:label "Liquid"@en ;
  rdfs:comment "The composite of the EuroWordNet Concepts Liquid."@en .
:Liquid-Artifact a :ConceptComposite ;
  rdfs:label "Liquid-Artifact"@en ;
  rdfs:comment "The composite of the EuroWordNet Concepts Liquid-Artifact."@en .
:Liquid-Natural a :ConceptComposite ;
  rdfs:label "Liquid-Natural"@en ;
  rdfs:comment "The composite of the EuroWordNet Concepts Liquid-Natural."@en .
:Living-Object a :ConceptComposite ;
  rdfs:label "Living-Object"@en ;
  rdfs:comment "The composite of the EuroWordNet Concepts Living-Object."@en .
:MoneyRepresentation a :ConceptComposite ;
  rdfs:label "MoneyRepresentation"@en ;
  rdfs:comment "The composite of the EuroWordNet Concepts MoneyRepresentation."@en .
:Natural-Group a :ConceptComposite ;
  rdfs:label "Natural-Group"@en ;
  rdfs:comment "The composite of the EuroWordNet Concepts Natural-Group."@en .
:Natural-Object a :ConceptComposite ;
  rdfs:label "Natural-Object"@en ;
  rdfs:comment "The composite of the EuroWordNet Concepts Natural-Object."@en .
:Natural-Object-BodyPart a :ConceptComposite ;
  rdfs:label "Natural-Object-BodyPart"@en ;
  rdfs:comment "The composite of the EuroWordNet Concepts Natural-Object-BodyPart."@en .
:Natural-Object-Part a :ConceptComposite ;
  rdfs:label "Natural-Object-Part"@en ;
  rdfs:comment "The composite of the EuroWordNet Concepts Natural-Object-Part."@en .
:Natural-Substance a :ConceptComposite ;
  rdfs:label "Natural-Substance"@en ;
  rdfs:comment "The composite of the EuroWordNet Concepts Natural-Substance."@en .
:Natural-Substance-Part a :ConceptComposite ;
  rdfs:label "Natural-Substance-Part"@en ;
  rdfs:comment "The composite of the EuroWordNet Concepts Natural-Substance-Part."@en .
:Object a :ConceptComposite ;
  rdfs:label "Object"@en ;
  rdfs:comment "The composite of the EuroWordNet Concepts Object."@en .
:Object-Part a :ConceptComposite ;
  rdfs:label "Object-Part"@en ;
  rdfs:comment "The composite of the EuroWordNet Concepts Object-Part."@en .
:Part a :ConceptComposite ;
  rdfs:label "Part"@en ;
  rdfs:comment "The composite of the EuroWordNet Concepts Part."@en .
:Place a :ConceptComposite ;
  rdfs:label "Place"@en ;
  rdfs:comment "The composite of the EuroWordNet Concepts Place."@en .
:Place-Liquid-Natural a :ConceptComposite ;
  rdfs:label "Place-Liquid-Natural"@en ;
  rdfs:comment "The composite of the EuroWordNet Concepts Place-Liquid-Natural."@en .
:Place-Object a :ConceptComposite ;
  rdfs:label "Place-Object"@en ;
  rdfs:comment "The composite of the EuroWordNet Concepts Place-Object."@en .
:Place-Object-Artifact a :ConceptComposite ;
  rdfs:label "Place-Object-Artifact"@en ;
  rdfs:comment "The composite of the EuroWordNet Concepts Place-Object-Artifact."@en .
:Place-Object-Artifact-Part a :ConceptComposite ;
  rdfs:label "Place-Object-Artifact-Part"@en ;
  rdfs:comment "The composite of the EuroWordNet Concepts Place-Object-Artifact-Part."@en .
:Place-Object-Group a :ConceptComposite ;
  rdfs:label "Place-Object-Group"@en ;
  rdfs:comment "The composite of the EuroWordNet Concepts Place-Object-Group."@en .
:Place-Object-Natural a :ConceptComposite ;
  rdfs:label "Place-Object-Natural"@en ;
  rdfs:comment "The composite of the EuroWordNet Concepts Place-Object-Natural."@en .
:Place-Object-Natural-Part a :ConceptComposite ;
  rdfs:label "Place-Object-Natural-Part"@en ;
  rdfs:comment "The composite of the EuroWordNet Concepts Place-Object-Natural-Part."@en .
:Place-Object-Part a :ConceptComposite ;
  rdfs:label "Place-Object-Part"@en ;
  rdfs:comment "The composite of the EuroWordNet Concepts Place-Object-Part."@en .
:Plant-Group a :ConceptComposite ;
  rdfs:label "Plant-Group"@en ;
  rdfs:comment "The composite of the EuroWordNet Concepts Plant-Group."@en .
:Plant-Object a :ConceptComposite ;
  rdfs:label "Plant-Object"@en ;
  rdfs:comment "The composite of the EuroWordNet Concepts Plant-Object."@en .
:Plant-Object-Comestible a :ConceptComposite ;
  rdfs:label "Plant-Object-Comestible"@en ;
  rdfs:comment "The composite of the EuroWordNet Concepts Plant-Object-Comestible."@en .
:Plant-Object-Part a :ConceptComposite ;
  rdfs:label "Plant-Object-Part"@en ;
  rdfs:comment "The composite of the EuroWordNet Concepts Plant-Object-Part."@en .
:Plant-Object-Part-Comestible a :ConceptComposite ;
  rdfs:label "Plant-Object-Part-Comestible"@en ;
  rdfs:comment "The composite of the EuroWordNet Concepts Plant-Object-Part-Comestible."@en .
:Property a :ConceptComposite ;
  rdfs:label "Property"@en ;
  rdfs:comment "The composite of the EuroWordNet Concepts Property."@en .
:Property-Existence a :ConceptComposite ;
  rdfs:label "Property-Existence"@en ;
  rdfs:comment "The composite of the EuroWordNet Concepts Property-Existence."@en .
:Property-LanguageRepresentation a :ConceptComposite ;
  rdfs:label "Property-LanguageRepresentation"@en ;
  rdfs:comment "The composite of the EuroWordNet Concepts Property-LanguageRepresentation."@en .
:Property-Location a :ConceptComposite ;
  rdfs:label "Property-Location"@en ;
  rdfs:comment "The composite of the EuroWordNet Concepts Property-Location."@en .
:Property-Mental a :ConceptComposite ;
  rdfs:label "Property-Mental"@en ;
  rdfs:comment "The composite of the EuroWordNet Concepts Property-Mental."@en .
:Property-Physical a :ConceptComposite ;
  rdfs:label "Property-Physical"@en ;
  rdfs:comment "The composite of the EuroWordNet Concepts Property-Physical."@en .
:Property-Physical-Colour a :ConceptComposite ;
  rdfs:label "Property-Physical-Colour"@en ;
  rdfs:comment "The composite of the EuroWordNet Concepts Property-Physical-Colour."@en .
:Property-Physical-Condition a :ConceptComposite ;
  rdfs:label "Property-Physical-Condition"@en ;
  rdfs:comment "The composite of the EuroWordNet Concepts Property-Physical-Condition."@en .
:Property-Physical-Form a :ConceptComposite ;
  rdfs:label "Property-Physical-Form"@en ;
  rdfs:comment "The composite of the EuroWordNet Concepts Property-Physical-Form."@en .
:Property-Social a :ConceptComposite ;
  rdfs:label "Property-Social"@en ;
  rdfs:comment "The composite of the EuroWordNet Concepts Property-Social."@en .
:Property-Stimulating-Physical a :ConceptComposite ;
  rdfs:label "Property-Stimulating-Physical"@en ;
  rdfs:comment "The composite of the EuroWordNet Concepts Property-Stimulating-Physical."@en .
:Property-Time a :ConceptComposite ;
  rdfs:label "Property-Time"@en ;
  rdfs:comment "The composite of the EuroWordNet Concepts Property-Time."@en .
:Relation a :ConceptComposite ;
  rdfs:label "Relation"@en ;
  rdfs:comment "The composite of the EuroWordNet Concepts Relation."@en .
:Relation-Location a :ConceptComposite ;
  rdfs:label "Relation-Location"@en ;
  rdfs:comment "The composite of the EuroWordNet Concepts Relation-Location."@en .
:Relation-Possession a :ConceptComposite ;
  rdfs:label "Relation-Possession"@en ;
  rdfs:comment "The composite of the EuroWordNet Concepts Relation-Possession."@en .
:Representation a :ConceptComposite ;
  rdfs:label "Representation"@en ;
  rdfs:comment "The composite of the EuroWordNet Concepts Representation."@en .
:SecondOrderEntity a :ConceptComposite ;
  rdfs:label "SecondOrderEntity"@en ;
  rdfs:comment "The composite of the EuroWordNet Concepts SecondOrderEntity."@en .
:Software a :ConceptComposite ;
  rdfs:label "Software"@en ;
  rdfs:comment "The composite of the EuroWordNet Concepts Software."@en .
:Static a :ConceptComposite ;
  rdfs:label "Static"@en ;
  rdfs:comment "The composite of the EuroWordNet Concepts Static."@en .
:Static-Existence a :ConceptComposite ;
  rdfs:label "Static-Existence"@en ;
  rdfs:comment "The composite of the EuroWordNet Concepts Static-Existence."@en .
:Static-Location a :ConceptComposite ;
  rdfs:label "Static-Location"@en ;
  rdfs:comment "The composite of the EuroWordNet Concepts Static-Location."@en .
:Static-Mental a :ConceptComposite ;
  rdfs:label "Static-Mental"@en ;
  rdfs:comment "The composite of the EuroWordNet Concepts Static-Mental."@en .
:Static-Relation a :ConceptComposite ;
  rdfs:label "Static-Relation"@en ;
  rdfs:comment "The composite of the EuroWordNet Concepts Static-Relation."@en .
:Static-Social a :ConceptComposite ;
  rdfs:label "Static-Social"@en ;
  rdfs:comment "The composite of the EuroWordNet Concepts Static-Social."@en .
:Substance a :ConceptComposite ;
  rdfs:label "Substance"@en ;
  rdfs:comment "The composite of the EuroWordNet Concepts Substance."@en .
:ThirdOrderEntity a :ConceptComposite ;
  rdfs:label "ThirdOrderEntity"@en ;
  rdfs:comment "The composite of the EuroWordNet Concepts ThirdOrderEntity."@en .
:ThirdOrderEntity-Mental a :ConceptComposite ;
  rdfs:label "ThirdOrderEntity-Mental"@en ;
  rdfs:comment "The composite of the EuroWordNet Concepts ThirdOrderEntity-Mental."@en .
:ThirdOrderEntity-Mental-Experience a :ConceptComposite ;
  rdfs:label "ThirdOrderEntity-Mental-Experience"@en ;
  rdfs:comment "The composite of the EuroWordNet Concepts ThirdOrderEntity-Mental-Experience."@en .
:ThirdOrderEntity-Mental-Location a :ConceptComposite ;
  rdfs:label "ThirdOrderEntity-Mental-Location"@en ;
  rdfs:comment "The composite of the EuroWordNet Concepts ThirdOrderEntity-Mental-Location."@en .
:ThirdOrderEntity-Mental-Purpose a :ConceptComposite ;
  rdfs:label "ThirdOrderEntity-Mental-Purpose"@en ;
  rdfs:comment "The composite of the EuroWordNet Concepts ThirdOrderEntity-Mental-Purpose."@en .
:ThirdOrderEntity-Mental-Purpose-Domain a :ConceptComposite ;
  rdfs:label "ThirdOrderEntity-Mental-Purpose-Domain"@en ;
  rdfs:comment "The composite of the EuroWordNet Concepts ThirdOrderEntity-Mental-Purpose-Domain."@en .
:ThirdOrderEntity-Mental-Purpose-Manner a :ConceptComposite ;
  rdfs:label "ThirdOrderEntity-Mental-Purpose-Manner"@en ;
  rdfs:comment "The composite of the EuroWordNet Concepts ThirdOrderEntity-Mental-Purpose-Manner."@en .
:ThirdOrderEntity-Mental-Purpose-Social a :ConceptComposite ;
  rdfs:label "ThirdOrderEntity-Mental-Purpose-Social"@en ;
  rdfs:comment "The composite of the EuroWordNet Concepts ThirdOrderEntity-Mental-Purpose-Social."@en .
:ThirdOrderEntity-Mental-Purpose-Social-Institution a :ConceptComposite ;
  rdfs:label "ThirdOrderEntity-Mental-Purpose-Social-Institution"@en ;
  rdfs:comment "The composite of the EuroWordNet Concepts ThirdOrderEntity-Mental-Purpose-Social-Institution."@en .
:ThirdOrderEntity-Mental-Social a :ConceptComposite ;
  rdfs:label "ThirdOrderEntity-Mental-Social"@en ;
  rdfs:comment "The composite of the EuroWordNet Concepts ThirdOrderEntity-Mental-Social."@en .
:ThirdOrderEntity-Part a :ConceptComposite ;
  rdfs:label "ThirdOrderEntity-Part"@en ;
  rdfs:comment "The composite of the EuroWordNet Concepts ThirdOrderEntity-Part."@en .
:ThirdOrderEntity-Quantity a :ConceptComposite ;
  rdfs:label "ThirdOrderEntity-Quantity"@en ;
  rdfs:comment "The composite of the EuroWordNet Concepts ThirdOrderEntity-Quantity."@en .
:ThirdOrderEntity-Quantity-MoneyRepresentation a :ConceptComposite ;
  rdfs:label "ThirdOrderEntity-Quantity-MoneyRepresentation"@en ;
  rdfs:comment "The composite of the EuroWordNet Concepts ThirdOrderEntity-Quantity-MoneyRepresentation."@en .
:ThirdOrderEntity-Quantity-Part a :ConceptComposite ;
  rdfs:label "ThirdOrderEntity-Quantity-Part"@en ;
  rdfs:comment "The composite of the EuroWordNet Concepts ThirdOrderEntity-Quantity-Part."@en .
:ThirdOrderEntity-Relation a :ConceptComposite ;
  rdfs:label "ThirdOrderEntity-Relation"@en ;
  rdfs:comment "The composite of the EuroWordNet Concepts ThirdOrderEntity-Relation."@en .
:ThirdOrderEntity-Time a :ConceptComposite ;
  rdfs:label "ThirdOrderEntity-Time"@en ;
  rdfs:comment "The composite of the EuroWordNet Concepts ThirdOrderEntity-Time."@en .
:ThirdOrderEntity-Time-Part a :ConceptComposite ;
  rdfs:label "ThirdOrderEntity-Time-Part"@en ;
  rdfs:comment "The composite of the EuroWordNet Concepts ThirdOrderEntity-Time-Part."@en .
:UnboundedEvent a :ConceptComposite ;
  rdfs:label "UnboundedEvent"@en ;
  rdfs:comment "The composite of the EuroWordNet Concepts UnboundedEvent."@en .
:UnboundedEvent-Agentive a :ConceptComposite ;
  rdfs:label "UnboundedEvent-Agentive"@en ;
  rdfs:comment "The composite of the EuroWordNet Concepts UnboundedEvent-Agentive."@en .
:UnboundedEvent-Agentive-Communication-Social a :ConceptComposite ;
  rdfs:label "UnboundedEvent-Agentive-Communication-Social"@en ;
  rdfs:comment "The composite of the EuroWordNet Concepts UnboundedEvent-Agentive-Communication-Social."@en .
:UnboundedEvent-Agentive-Existence a :ConceptComposite ;
  rdfs:label "UnboundedEvent-Agentive-Existence"@en ;
  rdfs:comment "The composite of the EuroWordNet Concepts UnboundedEvent-Agentive-Existence."@en .
:UnboundedEvent-Agentive-Mental a :ConceptComposite ;
  rdfs:label "UnboundedEvent-Agentive-Mental"@en ;
  rdfs:comment "The composite of the EuroWordNet Concepts UnboundedEvent-Agentive-Mental."@en .
:UnboundedEvent-Agentive-Physical a :ConceptComposite ;
  rdfs:label "UnboundedEvent-Agentive-Physical"@en ;
  rdfs:comment "The composite of the EuroWordNet Concepts UnboundedEvent-Agentive-Physical."@en .
:UnboundedEvent-Agentive-Physical-Location a :ConceptComposite ;
  rdfs:label "UnboundedEvent-Agentive-Physical-Location"@en ;
  rdfs:comment "The composite of the EuroWordNet Concepts UnboundedEvent-Agentive-Physical-Location."@en .
:UnboundedEvent-Agentive-Physical-Purpose a :ConceptComposite ;
  rdfs:label "UnboundedEvent-Agentive-Physical-Purpose"@en ;
  rdfs:comment "The composite of the EuroWordNet Concepts UnboundedEvent-Agentive-Physical-Purpose."@en .
:UnboundedEvent-Agentive-Physical-Social a :ConceptComposite ;
  rdfs:label "UnboundedEvent-Agentive-Physical-Social"@en ;
  rdfs:comment "The composite of the EuroWordNet Concepts UnboundedEvent-Agentive-Physical-Social."@en .
:UnboundedEvent-Agentive-Purpose a :ConceptComposite ;
  rdfs:label "UnboundedEvent-Agentive-Purpose"@en ;
  rdfs:comment "The composite of the EuroWordNet Concepts UnboundedEvent-Agentive-Purpose."@en .
:UnboundedEvent-Cause a :ConceptComposite ;
  rdfs:label "UnboundedEvent-Cause"@en ;
  rdfs:comment "The composite of the EuroWordNet Concepts UnboundedEvent-Cause."@en .
:UnboundedEvent-Cause-Physical a :ConceptComposite ;
  rdfs:label "UnboundedEvent-Cause-Physical"@en ;
  rdfs:comment "The composite of the EuroWordNet Concepts UnboundedEvent-Cause-Physical."@en .
:UnboundedEvent-Cause-Physical-Location a :ConceptComposite ;
  rdfs:label "UnboundedEvent-Cause-Physical-Location"@en ;
  rdfs:comment "The composite of the EuroWordNet Concepts UnboundedEvent-Cause-Physical-Location."@en .
:UnboundedEvent-Communication-Purpose-Social a :ConceptComposite ;
  rdfs:label "UnboundedEvent-Communication-Purpose-Social"@en ;
  rdfs:comment "The composite of the EuroWordNet Concepts UnboundedEvent-Communication-Purpose-Social."@en .
:UnboundedEvent-Experience-Physical a :ConceptComposite ;
  rdfs:label "UnboundedEvent-Experience-Physical"@en ;
  rdfs:comment "The composite of the EuroWordNet Concepts UnboundedEvent-Experience-Physical."@en .
:UnboundedEvent-Mental a :ConceptComposite ;
  rdfs:label "UnboundedEvent-Mental"@en ;
  rdfs:comment "The composite of the EuroWordNet Concepts UnboundedEvent-Mental."@en .
:UnboundedEvent-Phenomenal a :ConceptComposite ;
  rdfs:label "UnboundedEvent-Phenomenal"@en ;
  rdfs:comment "The composite of the EuroWordNet Concepts UnboundedEvent-Phenomenal."@en .
:UnboundedEvent-Phenomenal-Physical a :ConceptComposite ;
  rdfs:label "UnboundedEvent-Phenomenal-Physical"@en ;
  rdfs:comment "The composite of the EuroWordNet Concepts UnboundedEvent-Phenomenal-Physical."@en .
:UnboundedEvent-Physical-Location a :ConceptComposite ;
  rdfs:label "UnboundedEvent-Physical-Location"@en ;
  rdfs:comment "The composite of the EuroWordNet Concepts UnboundedEvent-Physical-Location."@en .
:UnboundedEvent-Social a :ConceptComposite ;
  rdfs:label "UnboundedEvent-Social"@en ;
  rdfs:comment "The composite of the EuroWordNet Concepts UnboundedEvent-Social."@en .
:UnboundedEvent-Time a :ConceptComposite ;
  rdfs:label "UnboundedEvent-Time"@en ;
  rdfs:comment "The composite of the EuroWordNet Concepts UnboundedEvent-Time."@en .
:Underspecified a :ConceptComposite ;
  rdfs:label "Underspecified"@en ;
  rdfs:comment "The composite of the EuroWordNet Concepts Underspecified."@en .
:Vehicle-Object-Artifact a :ConceptComposite ;
  rdfs:label "Vehicle-Object-Artifact"@en ;
  rdfs:comment "The composite of the EuroWordNet Concepts Vehicle-Object-Artifact."@en .
:Vehicle-Object-Artifact-Group a :ConceptComposite ;
  rdfs:label "Vehicle-Object-Artifact-Group"@en ;
  rdfs:comment "The composite of the EuroWordNet Concepts Vehicle-Object-Artifact-Group."@en .
:Vehicle-Object-Artifact-Part a :ConceptComposite ;
  rdfs:label "Vehicle-Object-Artifact-Part"@en ;
  rdfs:comment "The composite of the EuroWordNet Concepts Vehicle-Object-Artifact-Part."@en .
