@prefix : <http://www.wordnet.dk/dannet/2022/schema/> .
@prefix dnc: <http://www.wordnet.dk/dannet/2022/concepts/> .
@prefix ontolex: <http://www.w3.org/ns/lemon/ontolex#> .
@prefix owl: <http://www.w3.org/2002/07/owl#> .
@prefix rdfs: <http://www.w3.org/2000/01/rdf-schema#> .

:orthogonalHypernym a owl:ObjectProperty ;
  rdfs:domain ontolex:LexicalConcept ;
  rdfs:range ontolex:LexicalConcept ;
  rdfs:comment "Hypernyms that are orthogonal to the taxonomy; see: <https://cst.ku.dk/projekter/dannet/#heading-1612789460891>"@en ;
  rdfs:label "Orthogonal hypernym"@en ;
  owl:inverseOf :orthogonalHyponym .

:orthogonalHyponym a owl:ObjectProperty ;
  rdfs:domain ontolex:LexicalConcept ;
  rdfs:range ontolex:LexicalConcept ;
  rdfs:comment "Hyponyms that are orthogonal to the taxonomy; see: <https://cst.ku.dk/projekter/dannet/#heading-1612789460891>"@en ;
  rdfs:label "Orthogonal hyponym"@en ;
  owl:inverseOf :orthogonalHypernym .

:ontologicalFacet a owl:ObjectProperty ;
  rdfs:domain ontolex:LexicalConcept ;
  rdfs:range :Concept ;
  rdfs:comment "The DanNet/EuroWordNet Concept describing a facet of the synset."@en ;
  rdfs:label "Ontological facet"@en .

:ontologicalType a owl:ObjectProperty ;
  rdfs:domain ontolex:LexicalConcept ;
  rdfs:range :ConceptComposite ;
  rdfs:comment "The DanNet/EuroWordNet concept composite describing multiple facets of the synset."@en ;
  rdfs:label "Ontological type"@en .

:Concept a owl:Class ;
  rdfs:label "Concept"@en ;
  rdfs:comment "A concept found in either DanNet or EuroWordNet."@en .

:DanNetConcept a owl:Class ;
  rdfs:subClassOf :Concept ;
  rdfs:label "DanNet Concept"@en ;
  rdfs:comment "A concept created specifically for DanNet that extends the concepts from EuroWordNet; see: <https://cst.ku.dk/projekter/dannet/#heading-1612789460891>."@en .

:EuroWordNetConcept a owl:Class ;
  rdfs:subClassOf :Concept ;
  rdfs:label "EuroWordNet concept"@en ;
  rdfs:comment "A concept based on the 1st, 2nd, and 3rd order entities from EuroWordNet; see: <https://archive.illc.uva.nl/EuroWordNet/corebcs/topont.html>."@en .

:ConceptComposite a owl:Class ;
  rdfs:label "DanNet/EuroWordNet concept composite"@en ;
  rdfs:comment "A composite of one or more concepts from DanNet/EuroWordNet used to categorize synsets in DanNet; see: <https://cst.ku.dk/projekter/dannet/#heading-1612789460891>."@en .
