@prefix : <https://wordnet.dk/dannet/schema/> .
@prefix dnc: <https://wordnet.dk/dannet/concepts/> .
@prefix ontolex: <http://www.w3.org/ns/lemon/ontolex#> .
@prefix owl: <http://www.w3.org/2002/07/owl#> .
@prefix rdf: <http://www.w3.org/1999/02/22-rdf-syntax-ns#> .
@prefix rdfs: <http://www.w3.org/2000/01/rdf-schema#> .
@prefix skos: <http://www.w3.org/2004/02/skos/core#> .
@prefix marl: <http://www.gsi.upm.es/ontologies/marl/ns#> .
@prefix vann: <http://purl.org/vocab/vann/> .
@prefix xsd: <http://www.w3.org/2001/XMLSchema#> .
@prefix dc: <http://purl.org/dc/terms/> .
@prefix foaf: <http://xmlns.com/foaf/0.1/> .
@prefix dcat: <http://www.w3.org/ns/dcat#> .
@prefix wn: <https://globalwordnet.github.io/schemas/wn#> .

<https://wordnet.dk/dannet/schema> a owl:Ontology ;
  dc:issued "2023-09-08" ;
  dc:title "DanNet-skema"@da, "DanNet schema"@en;
  dc:description "Skema for DanNet-specifikke relationer."@da, "Schema for DanNet-specific relations."@en ;
  dc:publisher "<https://cst.dk>";
  vann:preferredNamespacePrefix "dns";
  vann:preferredNamespaceUri "https://wordnet.dk/dannet/schema/";
  foaf:homepage "<https://cst.ku.dk/projekter/dannet>";
  dc:license "<https://creativecommons.org/licenses/by-sa/4.0/>";
  dcat:downloadURL "<https://wordnet.dk/schema/dns>";
  dc:title "DanNet-skema"@da, "DanNet schema"@en;
  dc:rights "Copyright © Centre for Language Technology (University of Copenhagen) & The Society for Danish Language and Literature."@en, "Copyright © Center for Sprogteknologi (Københavns Universitet) & Det Danske Sprog- og Litteraturselskab."@da;
  dc:contributor "<https://simongray.dk>", "<https://cst.dk>", "<https://dsl.dk>";
  rdfs:seeAlso "<https://wordnet.dk/dannet/concepts>", "<https://wordnet.dk/dannet/data>" .

# NOTE: the format of :eq_hypernym and :eq_hyponym is a copy of wn:eq_synonym
:eqHypernym a wn:SynsetRelType ;
  rdfs:label "eq hypernym"@en ;
  rdfs:comment "A relation between two concepts in separate data sets where the object is a hypernym of the subject."@en ;
  rdfs:comment "En relation mellem to begreber i separate datasæt, hvor objektet er et hypernym af subjektet."@da ;
  owl:inverseOf :eqHyponym .

:eqHyponym a wn:SynsetRelType ;
  rdfs:label "eq hyponym"@en ;
  rdfs:comment "A relation between two concepts in separate data sets where the object is a hyponym of the subject."@en ;
  rdfs:comment "En relation mellem to begreber i separate datasæt, hvor objektet er et hyponym af subjektet."@da ;
  owl:inverseOf :eqHypernym .

:eqSimilar a wn:SynsetRelType ;
  rdfs:label "eq similar"@en ;
  rdfs:comment "A relation between two concepts in separate data sets where the object is similar to the subject, though not synonymous."@en ;
  rdfs:comment "En relation mellem to begreber i separate datasæt, hvor objektet minder om subjektet men dog ikke er et synonym."@da ;
  owl:inverseOf :eqSimilar .

# Infer inverse links from the ILI dataset for better navigation of the graph.
:linkedConcept a owl:ObjectProperty ;
  rdfs:label "linked concept"@en ;
  rdfs:label "forbundet begreb"@da ;
  rdfs:comment "The outgoing link to a lexical concept/synset from its designated Interlingual Index."@en ;
  rdfs:comment "Den udgående forbindelse til et leksikalsk begreb/synset fra dets noterede Interlingual Index."@da ;
  owl:inverseOf wn:ili .

:Gender a owl:Class .

:Male a owl:Class ;
  rdfs:label "male"@en ;
  rdfs:label "mand"@da ;
  rdfs:subClassOf :Gender .

:Female a owl:Class ;
  rdfs:label "female"@en ;
  rdfs:label "kvinde"@da ;
  rdfs:subClassOf :Gender .

:gender a owl:ObjectProperty ;
  rdfs:label "gender"@en ;
  rdfs:label "køn"@da ;
  rdfs:comment "The gender of the subject."@en ;
  rdfs:comment "Subjektets køn."@da ;
  rdfs:range :Gender .

:sentiment a owl:ObjectProperty ;
  rdfs:range marl:Opinion ;
  rdfs:label "sentiment"@en ;
  rdfs:label "stemning"@da ;
  rdfs:isDefinedBy <https://wordnet.dk/dannet/schema> .

:Inheritance a owl:Class ;
  rdfs:label "inheritance"@en ;
  rdfs:label "nedarvning"@da ;
  rdfs:comment "Meta-property documenting inherited relations in DanNet."@en ;
  rdfs:comment "Meta-egenskab der dokumenterer nedarvede relationer i DanNet."@da ;
  rdfs:isDefinedBy <https://wordnet.dk/dannet/schema> .

:inherited a owl:ObjectProperty ;
  rdfs:domain ontolex:LexicalConcept ;
  rdfs:range :Inheritance ;
  rdfs:comment "Inherited concept-concept relation."@en ;
  rdfs:comment "Nedarvet begreb-begreb relation."@da ;
  rdfs:label "inherited"@en ;
  rdfs:label "nedarvet"@da ;
  rdfs:isDefinedBy <https://wordnet.dk/dannet/schema> .

:inheritedFrom a owl:ObjectProperty ;
  rdfs:domain :Inheritance ;
  rdfs:range owl:ObjectProperty ;
  rdfs:comment "Source of an inherited relation."@en ;
  rdfs:comment "Kilde til en nedarvet relation."@da ;
  rdfs:label "inherited from"@en ;
  rdfs:label "nedarvet fra"@da ;
  rdfs:isDefinedBy <https://wordnet.dk/dannet/schema> .

:inheritedRelation a owl:ObjectProperty ;
  rdfs:domain :Inheritance ;
  rdfs:range owl:ObjectProperty ;
  rdfs:comment "Relation inherited from other concept."@en ;
  rdfs:comment "Relation nedarvet fra andet begreb."@da ;
  rdfs:label "inherited relation"@en ;
  rdfs:label "nedarvet relation"@da ;
  rdfs:isDefinedBy <https://wordnet.dk/dannet/schema> .

:usedFor a wn:SynsetRelType ;
  rdfs:domain ontolex:LexicalConcept ;
  rdfs:range ontolex:LexicalConcept ;
  rdfs:comment "A lexical concept which the subject concept may be used for; see<https://wordnet.dk/dannet/schema> .https://cst.ku.dk/projekter/dannet/#heading-1612789460891>"@en ;
  rdfs:comment "Et leksikalsk begreb som subjekt-begrebet kan bruges til; se<https://wordnet.dk/dannet/schema> .https://cst.ku.dk/projekter/dannet/#heading-1612789460891>"@da ;
  rdfs:label "used for"@en ;
  rdfs:label "brugt til"@da ;
  rdfs:isDefinedBy <https://wordnet.dk/dannet/schema> .

:usedForObject a wn:SynsetRelType ;
  rdfs:domain ontolex:LexicalConcept ;
  rdfs:range ontolex:LexicalConcept ;
  rdfs:comment "TODO; see<https://wordnet.dk/dannet/schema> .https://cst.ku.dk/projekter/dannet/#heading-1612789460891>"@en ;
  rdfs:comment "TODO; se<https://wordnet.dk/dannet/schema> .https://cst.ku.dk/projekter/dannet/#heading-1612789460891>"@da ;
  rdfs:label "used for object"@en ;
  rdfs:label "brugt til objekt"@da ;
  rdfs:isDefinedBy <https://wordnet.dk/dannet/schema> .

:nearAntonym a wn:SynsetRelType ;
  rdfs:domain ontolex:LexicalConcept ;
  rdfs:range ontolex:LexicalConcept ;
  rdfs:comment "A lexical concept which is a near antonym of the subject concept; see<https://wordnet.dk/dannet/schema> .https://cst.ku.dk/projekter/dannet/#heading-1612789460891>"@en ;
  rdfs:comment "Et leksikalsk begreb som er et nær-antonym af subjekt-begrebet; se<https://wordnet.dk/dannet/schema> .https://cst.ku.dk/projekter/dannet/#heading-1612789460891>"@da ;
  rdfs:label "near antonym"@en ;
  rdfs:label "nær-antonym"@da ;
  owl:inverseOf :nearAntonym ;
  rdfs:isDefinedBy <https://wordnet.dk/dannet/schema> .

:orthogonalHypernym a wn:SynsetRelType ;
  rdfs:domain ontolex:LexicalConcept ;
  rdfs:range ontolex:LexicalConcept ;
  rdfs:comment "Hypernyms that are orthogonal to the taxonomy; see<https://wordnet.dk/dannet/schema> .https://cst.ku.dk/projekter/dannet/#heading-1612789460891>"@en ;
  rdfs:comment "Hyperonymer der er ortogonale i taxonomien; se<https://wordnet.dk/dannet/schema> .https://cst.ku.dk/projekter/dannet/#heading-1612789460891>"@da ;
  rdfs:label "orthogonal hypernym"@en ;
  rdfs:label "ortogonalt hyperonym"@da ;
  owl:inverseOf :orthogonalHyponym ;
  rdfs:isDefinedBy <https://wordnet.dk/dannet/schema> .

:orthogonalHyponym a wn:SynsetRelType ;
  rdfs:domain ontolex:LexicalConcept ;
  rdfs:range ontolex:LexicalConcept ;
  rdfs:comment "Hyponyms that are orthogonal to the taxonomy; see<https://wordnet.dk/dannet/schema> .https://cst.ku.dk/projekter/dannet/#heading-1612789460891>"@en ;
  rdfs:comment "Hyponymer der er ortogonale i taxonomien; se<https://wordnet.dk/dannet/schema> .https://cst.ku.dk/projekter/dannet/#heading-1612789460891>"@da ;
  rdfs:label "orthogonal hyponym"@en ;
  rdfs:label "ortogonalt hyponym"@da ;
  owl:inverseOf :orthogonalHypernym ;
  rdfs:isDefinedBy <https://wordnet.dk/dannet/schema> .

:ontologicalType a owl:ObjectProperty ;
  rdfs:domain ontolex:LexicalConcept ;
  rdfs:range :OntologicalConcept ;
  rdfs:comment "A DanNet/EuroWordNet Concept describing a facet of a synset."@en ;
  rdfs:comment "Et DanNet/EuroWordNet-koncept der beskriver en facet af et synset."@da ;
  rdfs:label "ontological type"@en ;
  rdfs:label "ontologisk type"@da ;
  rdfs:isDefinedBy <https://wordnet.dk/dannet/schema> .

:OntologicalConcept a owl:Class ;
  rdfs:label "ontological concept"@en ;
  rdfs:label "ontologisk koncept"@da ;
  rdfs:comment "An ontological concept found in either DanNet or EuroWordNet."@en ;
  rdfs:comment "Et ontologisk koncept fundet i enten DanNet eller EuroWordNet."@da ;
  rdfs:isDefinedBy <https://wordnet.dk/dannet/schema> .

:DanNetConcept a owl:Class ;
  rdfs:subClassOf :OntologicalConcept ;
  rdfs:label "DanNet concept"@en ;
  rdfs:label "DanNet-koncept"@da ;
  rdfs:comment "An ontological concept created specifically for DanNet extending the concepts from EuroWordNet; see<https://wordnet.dk/dannet/schema> .https://cst.ku.dk/projekter/dannet/#heading-1612789460891>."@en ;
  rdfs:comment "Et ontologisk koncept skabt specifikt til DanNet, som udvider konceptsættet fra EuroWordNet; se<https://wordnet.dk/dannet/schema> .https://cst.ku.dk/projekter/dannet/#heading-1612789460891>."@da ;
  rdfs:isDefinedBy <https://wordnet.dk/dannet/schema> .

:EuroWordNetConcept a owl:Class ;
  rdfs:subClassOf :OntologicalConcept ;
  rdfs:label "EuroWordNet concept"@en ;
  rdfs:label "EuroWordNet-koncept"@da ;
  rdfs:comment "An ontological concept based on the 1st, 2nd, and 3rd order entities from EuroWordNet; see<https://wordnet.dk/dannet/schema> .https://archive.illc.uva.nl/EuroWordNet/corebcs/topont.html>."@en ;
  rdfs:comment "Et ontologisk koncept baseret på første-, anden-, og tredjeordens-enhederne fra EuroWordNet; se<https://wordnet.dk/dannet/schema> .https://archive.illc.uva.nl/EuroWordNet/corebcs/topont.html>."@da ;
  rdfs:isDefinedBy <https://wordnet.dk/dannet/schema> .

# TODO: this relation should be replaced by a mature, standardised alternative
:ddoFrequency a owl:ObjectProperty ;
  rdfs:domain ontolex:LexicalConcept ;
  rdfs:label "DDO frequency"@en ;
  rdfs:label "DDO-frekvens"@da ;
  rdfs:isDefinedBy <https://wordnet.dk/dannet/schema> .
