@prefix dc: <http://purl.org/dc/terms/> .
@prefix marl: <http://www.gsi.upm.es/ontologies/marl/ns#> .
@prefix owl: <http://www.w3.org/2002/07/owl#> .
@prefix protege: <http://protege.stanford.edu/plugins/owl/protege#> .
@prefix prov: <http://www.w3.org/ns/prov#> .
@prefix provdc: <http://www.w3.org/ns/prov-dc#> .
@prefix rdf: <http://www.w3.org/1999/02/22-rdf-syntax-ns#> .
@prefix rdfs: <http://www.w3.org/2000/01/rdf-schema#> .
@prefix swrl: <http://www.w3.org/2003/11/swrl#> .
@prefix swrlb: <http://www.w3.org/2003/11/swrlb#> .
@prefix xml: <http://www.w3.org/XML/1998/namespace> .
@prefix xsd: <http://www.w3.org/2001/XMLSchema#> .
@prefix xsp: <http://www.owl-ontologies.com/2005/08/07/xsp.owl#> .
@prefix skos: <http://www.w3.org/2004/02/skos/core#> .


<http://www.gsi.upm.es/ontologies/marl/ns> a owl:Ontology ;
    rdfs:label "Marl Opinion Ontology"@en ;
    dc:description "Marl is an ontology designed to use for publishing the results of the opinion mining process in a form of structured data on the Web. The goal is to unify the access the numerical approximation of the opinion concept and allow extensive reasoning and search over multiple resources from different content providers."@en ;
    rdfs:comment "Marl is an ontology designed to use for publishing the results of the opinion mining process in a form of structured data on the Web. The goal is to unify the access the numerical approximation of the opinion concept and allow extensive reasoning and search over multiple resources from different content providers."@en ;
    rdfs:seeAlso "http://www.gsi.upm.es/ontologies/marl/ns#"^^xsd:string ;

    owl:priorVersion <http://www.gsi.upm.es/ontologies/marl/1.1> ;
    owl:versionInfo "1.2"^^xsd:string .

marl:aggregatesOpinion a owl:ObjectProperty ;
    rdfs:label "aggregatesOpinion"@en ;
    rdfs:comment "Indicates that the polarity described with the class is a calculation (eg. sum) of other opinions polarity (eg. aggregated opinion about the movie derived from many sentiments expressed in one text)."@en ;
    rdfs:domain marl:AggregatedOpinion ;
    rdfs:isDefinedBy "http://www.gsi.upm.es/ontologies/marl/ns#"^^xsd:string ;
    rdfs:range marl:Opinion .

marl:algorithm a owl:ObjectProperty ;
    rdfs:label "algorithm"^^xsd:string ;
    rdfs:comment "The algorithm used in the Sentiment Analysis."@en ;
    rdfs:domain marl:SentimentAnalysis ;
    rdfs:isDefinedBy "http://www.gsi.upm.es/ontologies/marl/ns#"^^xsd:string .

marl:algorithmConfidence a owl:DatatypeProperty ;
    rdfs:label "algorithmConfidence"@en ;
    rdfs:comment "A numerical value that describe how much the algorithm was confident of the assessment of the opinion (eg. how much the opinion matches a gives object/product)."@en ;
    rdfs:domain marl:Opinion ;
    rdfs:isDefinedBy "http://www.gsi.upm.es/ontologies/marl/ns#"^^xsd:string ;
    rdfs:range xsd:float .

marl:describesFeature a owl:ObjectProperty ;
    rdfs:label "describesFeature"@en ;
    rdfs:comment "Indicates a feature of an object or object part that the opinion refers to (eg. laptop battery life or laptop battery size etc.)."@en ;
    rdfs:domain marl:Opinion ;
    rdfs:isDefinedBy "http://www.gsi.upm.es/ontologies/marl/ns#"^^xsd:string .

marl:describesObject a owl:ObjectProperty ;
    rdfs:label "describesObject"@en ;
    rdfs:comment "Indicates the object that the opinion refers to."@en ;
    rdfs:domain marl:Opinion ;
    rdfs:isDefinedBy "http://www.gsi.upm.es/ontologies/marl/ns#"^^xsd:string .

marl:describesObjectPart a owl:ObjectProperty ;
    rdfs:label "describesObjectPart"@en ;
    rdfs:comment "Indicates a particular element or part of the object that the opinion refers to (eg. laptop screen or camera battery)."@en ;
    rdfs:domain marl:Opinion ;
    rdfs:isDefinedBy "http://www.gsi.upm.es/ontologies/marl/ns#"^^xsd:string .

marl:domain a owl:ObjectProperty ;
    rdfs:label "domain"^^xsd:string ;
    rdfs:domain marl:Opinion ;
    rdfs:isDefinedBy "http://www.gsi.upm.es/ontologies/marl/ns#"^^xsd:string .

marl:hasPolarity a owl:ObjectProperty ;
    rdfs:label "hasPolarity"@en ;
    rdfs:comment "Indicates if the opinion is positive/negative or neutral. Use instances of class marl:Polarity."@en ;
    rdfs:domain marl:Opinion ;
    rdfs:isDefinedBy "http://www.gsi.upm.es/ontologies/marl/ns#"^^xsd:string ;
    rdfs:range marl:Polarity .

marl:maxPolarityValue a owl:DatatypeProperty ;
    rdfs:label "algorithmConfidence"@en ;
    rdfs:comment "Maximal possible numerical value for the opinion."@en ;
    rdfs:domain marl:SentimentAnalysis ;
    rdfs:isDefinedBy "http://www.gsi.upm.es/ontologies/marl/ns#"^^xsd:string .

marl:minPolarityValue a owl:DatatypeProperty ;
    rdfs:label "minPolarityValue"@en ;
    rdfs:comment "Lowest possible numerical value of the opinion."@en ;
    rdfs:domain marl:SentimentAnalysis ;
    rdfs:isDefinedBy "http://www.gsi.upm.es/ontologies/marl/ns#"^^xsd:string .

marl:negativeOpinionCount a owl:DatatypeProperty ;
    rdfs:label "negativeOpinionCount"@en ;
    rdfs:comment "Amount of negative opinions aggregated."@en ;
    rdfs:domain marl:AggregatedOpinion ;
    rdfs:isDefinedBy "http://www.gsi.upm.es/ontologies/marl/ns#"^^xsd:string .

marl:neutralOpinionCount a owl:DatatypeProperty ;
    rdfs:label "neutralOpinionCount"@en ;
    rdfs:comment "Amount of neutral opinions aggregated."@en ;
    rdfs:domain marl:AggregatedOpinion ;
    rdfs:isDefinedBy "http://www.gsi.upm.es/ontologies/marl/ns#"^^xsd:string .

marl:opinionCount a owl:DatatypeProperty ;
    rdfs:label "opinionCount"@en ;
    rdfs:comment "Amount of all aggregated opinions."@en ;
    rdfs:domain marl:AggregatedOpinion ;
    rdfs:isDefinedBy "http://www.gsi.upm.es/ontologies/marl/ns#"^^xsd:string .

marl:opinionText a owl:DatatypeProperty ;
    rdfs:label "opinionText"@en ;
    rdfs:comment """The exact text extract that expresses the opinion. This can be used when entity/text pointed by extractedFrom contains many opinions.

For example extractedFrom can point to a comment that contains many opinions about a movie, each opinion should have a separate marl:Opinion and optionally an opinionText  property to indicate the specific text fragment of the comment."""@en ;
    rdfs:domain marl:Opinion ;
    rdfs:isDefinedBy "http://www.gsi.upm.es/ontologies/marl/ns#"^^xsd:string .

marl:polarityValue a owl:DatatypeProperty ;
    rdfs:label "polarityValue"@en ;
    rdfs:comment "A numerical representation of the polarity value. The recommended use is by specifying % by using a real number from 0..1. In case this is not feasible in a given solution use minOpinionValue and maxOpinionValue to provide additional information."@en ;
    rdfs:domain marl:Opinion ;
    rdfs:isDefinedBy "http://www.gsi.upm.es/ontologies/marl/ns#"^^xsd:string .

marl:positiveOpinionsCount a owl:DatatypeProperty ;
    rdfs:label "positiveOpinionCount"@en ;
    rdfs:comment "Amount of positive opinions aggregated."@en ;
    rdfs:domain marl:AggregatedOpinion ;
    rdfs:isDefinedBy "http://www.gsi.upm.es/ontologies/marl/ns#"^^xsd:string .

marl:source a owl:ObjectProperty ;
    rdfs:label "source"^^xsd:string ;
    rdfs:comment "Source from which the opinion was extracted (URL, Site, Entity...)"^^xsd:string ;
    rdfs:domain marl:SentimentAnalysis ;
    rdfs:isDefinedBy "http://www.gsi.upm.es/ontologies/marl/ns#"^^xsd:string .

marl:sourceText a owl:ObjectProperty ;
    rdfs:label "sourceText"^^xsd:string ;
    rdfs:comment "Text analysed"^^xsd:string ;
    rdfs:isDefinedBy "http://www.gsi.upm.es/ontologies/marl/ns#"^^xsd:string .

marl:Negative a marl:Polarity ;
    a skos:Concept ;
    skos:broader marl:Polarity ;
    rdfs:label "Negative"@en ;
    rdfs:comment "Negative polarity."@en ;
    rdfs:isDefinedBy "http://www.gsi.upm.es/ontologies/marl/ns#"^^xsd:string .

marl:Neutral a marl:Polarity ;
    a skos:Concept ;
    skos:broader marl:Polarity ;
    rdfs:label "Neutral"@en ;
    rdfs:comment "Neutral polarity"@en ;
    rdfs:isDefinedBy "http://www.gsi.upm.es/ontologies/marl/ns#"^^xsd:string .

marl:Positive a marl:Polarity ;
    a skos:Concept ;
    skos:broader marl:Polarity ;
    rdfs:label "Positive"@en ;
    rdfs:comment "Positive polarity"@en ;
    rdfs:isDefinedBy "http://www.gsi.upm.es/ontologies/marl/ns#"^^xsd:string .

marl:extractedFrom a owl:ObjectProperty ;
    rdfs:label "extractedFrom"@en ;
    rdfs:comment "Indicates the text from which the opinion has been extracted."@en ;
    rdfs:domain marl:Opinion ;
    rdfs:isDefinedBy "http://www.gsi.upm.es/ontologies/marl/ns#"^^xsd:string ;
    owl:inverseOf marl:hasOpinion .

marl:hasOpinion a owl:ObjectProperty ;
    rdfs:label "hasOpinion"@en ;
    rdfs:comment "Indicates that a certain text has a subjective opinion expressed in it."@en ;
    rdfs:isDefinedBy "http://www.gsi.upm.es/ontologies/marl/ns#"^^xsd:string ;
    rdfs:range marl:Opinion ;
    owl:inverseOf marl:extractedFrom .

marl:Polarity a owl:Class ;
              a skos:Concept ;
    rdfs:label "Polarity"@en ;
    rdfs:comment "Class that represents the opinion polarity. Use instances to express if the polarity is positive, neutral or negative."@en ;
    rdfs:isDefinedBy "http://www.gsi.upm.es/ontologies/marl/ns#"^^xsd:string .

marl:SentimentAnalysis a owl:Class ;
    rdfs:label "SentimentAnalysis"^^xsd:string ;
    rdfs:comment """<p style="margin-top: 0">
      The action of analysing the sentiment in an entity. It produces a
      marl:opinion
    </p>"""@en ;
    rdfs:isDefinedBy "http://www.gsi.upm.es/ontologies/marl/ns#"^^xsd:string ;
    rdfs:subClassOf prov:Activity .

marl:AggregatedOpinion a owl:Class ;
    rdfs:label "AggregatedOpinion"@en ;
    rdfs:comment "The same as Opinion class but indicates that the properties of this class aggregate all the opinions specified in the \"extractedFrom\" source. Optionally, if the aggregatesOpinion property is used this class could be created to aggregate only certain opinions (e.g. in a text about political scene it there could be many AggregatedOpinion classes each with opinions per different politician)."@en ;
    rdfs:isDefinedBy "http://www.gsi.upm.es/ontologies/marl/ns#"^^xsd:string ;
    rdfs:subClassOf marl:Opinion .

marl:Opinion a owl:Class ;
    rdfs:label "Opinion"@en ;
    rdfs:comment "Describes the concept of opinion expressed in a certain text."@en ;
    rdfs:isDefinedBy "http://www.gsi.upm.es/ontologies/marl/ns#"^^xsd:string ;
    rdfs:subClassOf prov:Entity .

[] a owl:AllDifferent ;
    owl:distinctMembers [ rdf:first marl:Negative ;
            rdf:rest [ rdf:first marl:Neutral ;
                    rdf:rest [ rdf:first marl:Positive ] ] ] .
